src/cbor/pulse/raw/everparse/CBOR.Pulse.Raw.EverParse.Validate.fsti
@@ -237,3 +237,15 @@ val impl_holds_on_raw_data_item
 : stt bool
   (requires pts_to_serialized serialize_raw_data_item input #pm v)
   (ensures fun res -> pts_to_serialized serialize_raw_data_item input #pm v ** pure (res == holds_on_raw_data_item p v))
+
+inline_for_extraction
+val impl_holds_on_raw_data_item_strong_prefix
+  (f64: squash SZ.fits_u64)
+  (p: Ghost.erased (raw_data_item -> bool))
+  (impl_p: LowParse.Pulse.Recursive.impl_pred_strong_prefix_t serialize_raw_data_item_param p)
+  (input: slice byte)
+  (#pm: perm)
+  (#v: Ghost.erased raw_data_item)
+: stt bool
+  (requires LowParse.PulseParse.Base.pts_to_parsed_strong_prefix parse_raw_data_item input #pm v)
+  (ensures fun res -> LowParse.PulseParse.Base.pts_to_parsed_strong_prefix parse_raw_data_item input #pm v ** pure (res == holds_on_raw_data_item p v))
